add IndRunner to help with induction equiv proofs
I intended to use these results in a proof of a forking lemma with
a standard RO (instead of FRO), but have since then came up with
a much simpler solution.

As a result, the added lemmas likely won't be used in the next
couple of commits, but for now, I want to keep them around, should
they become useful later.

proof/Stopping.ec
@@ -1,3 +1,4 @@
+pragma Goals:printall.
 require import AllCore.
 
 type query_t, resp_t.
@@ -54,3 +55,77 @@ module Runner(S : Stoppable, O : Oracle) = {
  *   declare module SAdv <: Stoppable.
  *   module Adv = Runner(SAdv).
  *)
+
+module IndRunner(S : Stoppable, O : Oracle) = {
+  proc iter(q : query_t, n : int) : query_t = {
+    var r : resp_t;
+
+    while (0 < n) {
+      r <@ O.get(q);
+      q <@ S.continue(r);
+      n <- n - 1;
+    }
+
+    return q;
+  }
+
+  proc init(i : in_t, n : int) : query_t = {
+    var q : query_t;
+    q <@ S.init(i);
+    q <@ iter(q, n - 1);
+    return q;
+  }
+
+  proc init_split(i : in_t, k : int, l : int) : query_t = {
+    var q : query_t;
+    q <@ init(i, k);
+    q <@ iter(q, l);
+    return q;
+  }
+
+  proc run(i : in_t, n : int) : out_t = {
+    var o : out_t;
+    var q : query_t;
+    var r : resp_t;
+
+    q <@ init(i, n);
+    r <@ O.get(q);
+    o <@ S.finish(r);
+
+    return o;
+  }
+}.
+
+section PROOF.
+
+declare module O <: Oracle.
+(* TODO: Can we avoid this restriction? *)
+declare module S <: Stoppable {-O}.
+
+equiv ind_run_equiv :
+  Runner(S, O).run ~ IndRunner(S, O).run :
+  (arg{1}, Q) = arg{2} /\ ={glob S, glob O} ==>
+  ={res, glob S, glob O}.
+proof.
+proc; inline.
+sim.
+while (={glob S, glob O} /\ q{1} = q1{2} /\ c{1} + n1{2} = Q).
++ wp; do 2! call (_ : true); skip => /#.
+wp; call (_ : true); wp; skip => /#.
+qed.
+
+equiv ind_split_equiv :
+  IndRunner(S, O).init ~ IndRunner(S, O).init_split :
+  ={glob S, glob O, i} /\ n{1} = k{2} + l{2} /\ 0 < k{2} /\ 0 <= l{2} ==>
+  ={res, glob S, glob O}.
+proof.
+proc => /=; inline.
+exlim k{2}, l{2} => k0 l0.
+splitwhile {1} 4 : 0 < n0 - l0.
+sim.
+while (={glob S, glob O} /\ q0{1} = q2{2} /\ n0{1} - l0 = n1{2} /\ 0 <= n1{2} /\ 0 <= l0).
++ wp; do 2! call (_ : true); skip => /#.
+wp; call (_ : true); wp; skip => /#.
+qed.
+
+end section PROOF.
